Capless/Subst/Capture/Subcapturing.lean
@@ -1,0 +1,10 @@
+import Capless.Subcapturing
+import Capless.Subst.Basic
+namespace Capless
+
+theorem Subcapt.csubst
+  (h : Subcapt Γ C1 C2)
+  (σ : CVarSubst Γ f Δ) :
+  Subcapt Δ (C1.crename f) (C2.crename f) := by sorry
+
+end Capless
