Capless/Subst/Capture/Typing.lean
@@ -1,0 +1,10 @@
+import Capless.Subtyping
+import Capless.Subst.Basic
+namespace Capless
+
+theorem Typed.csubst
+  (h : Typed Γ t E)
+  (σ : CVarSubst Γ f Δ) :
+  Typed Δ (t.crename f) (E.crename f) := by sorry
+
+end Capless
