Capless/Subst/Type/Subcapturing.lean
@@ -1,0 +1,10 @@
+import Capless.Subst.Basic
+import Capless.Subcapturing
+namespace Capless
+
+theorem Subcapt.tsubst
+  (h : Subcapt Γ C1 C2)
+  (σ : TVarSubst Γ f Δ) :
+  Subcapt Δ C1 C2 := by sorry
+
+end Capless
