Capless/Subst/Type/Subtyping.lean
@@ -1,0 +1,10 @@
+import Capless.Subst.Basic
+import Capless.Subtyping
+namespace Capless
+
+theorem SSubtyp.tsubst
+  (h : SSubtyp Γ S1 S2)
+  (σ : TVarSubst Γ f Δ) :
+  SSubtyp Δ (S1.trename f) (S2.trename f) := sorry
+
+end Capless
