Capless/Subst/Type/Typing.lean
@@ -1,0 +1,10 @@
+import Capless.Subst.Basic
+import Capless.Typing
+namespace Capless
+
+theorem Typed.tsubst
+  (h : Typed Γ t E)
+  (σ : TVarSubst Γ f Δ) :
+  Typed Δ (t.trename f) (E.trename f) := by sorry
+
+end Capless
